Prove msg_id_unique axiom!

src/Broadcast.thy
@@ -19,16 +19,16 @@ record ('nodeid, 'op) message =
 
 type_synonym ('nodeid, 'op) node_state = "(('nodeid, 'op) message event, unit) node"
 
-definition broadcasts :: "('nodeid, 'op) node_state \<Rightarrow> ('nodeid, 'op) message list" where
-  "broadcasts state \<equiv> List.map_filter (\<lambda>e. case e of Broadcast m \<Rightarrow> Some m | _ \<Rightarrow> None) (fst state)"
+definition filter_bcast :: "('nodeid, 'op) message event list \<Rightarrow> ('nodeid, 'op) message list" where
+  "filter_bcast evts \<equiv> List.map_filter (\<lambda>e. case e of Broadcast m \<Rightarrow> Some m | _ \<Rightarrow> None) evts"
 
-definition deliveries :: "('nodeid, 'op) node_state \<Rightarrow> ('nodeid, 'op) message list" where
-  "deliveries state \<equiv> List.map_filter (\<lambda>e. case e of Deliver m \<Rightarrow> Some m | _ \<Rightarrow> None) (fst state)"
+definition filter_deliv :: "('nodeid, 'op) message event list \<Rightarrow> ('nodeid, 'op) message list" where
+  "filter_deliv evts \<equiv> List.map_filter (\<lambda>e. case e of Deliver m \<Rightarrow> Some m | _ \<Rightarrow> None) evts"
 
 definition causal_deps :: "('nodeid, 'op) node_state \<Rightarrow> 'nodeid \<Rightarrow> nat" where
   "causal_deps state \<equiv> foldl
     (\<lambda>map msg. case msg_id msg of (node, seq) \<Rightarrow> map(node := seq))
-    (\<lambda>n. 0) (deliveries state)"
+    (\<lambda>n. 0) (filter_deliv (fst state))"
 
 definition deps_leq :: "('nodeid \<Rightarrow> nat) \<Rightarrow> ('nodeid \<Rightarrow> nat) \<Rightarrow> bool" where
   "deps_leq left right \<equiv> \<forall>node::'nodeid. left node \<le> right node"
@@ -39,7 +39,7 @@ definition causally_ready :: "('nodeid, 'op) node_state \<Rightarrow> ('nodeid, 
      (case msg_id msg of (sender, seq) \<Rightarrow> seq = Suc(causal_deps state sender))"
 
 definition next_msgid :: "'nodeid \<Rightarrow> ('nodeid, 'op) node_state \<Rightarrow> 'nodeid msgid" where
-  "next_msgid sender state \<equiv> (sender, Suc (length (broadcasts state)))"
+  "next_msgid sender state \<equiv> (sender, Suc (length (filter_bcast (fst state))))"
 
 definition valid_msgs :: "(('nodeid, 'op) node_state \<Rightarrow> 'op set) \<Rightarrow> 'nodeid \<Rightarrow> ('nodeid, 'op) node_state \<Rightarrow> ('nodeid, 'op) message set" where
   "valid_msgs valid_ops sender state \<equiv>
@@ -159,26 +159,24 @@ lemma (in cbcast_protocol) broadcast_msg_eq:
 done
 
 lemma (in cbcast_protocol) map_filter_broadcast:
-  assumes "msg \<in> set (List.map_filter
-           (\<lambda>e. case e of Broadcast m \<Rightarrow> Some m | _ \<Rightarrow> None) hist)"
+  assumes "msg \<in> set (filter_bcast hist)"
   shows "Broadcast msg \<in> set hist"
   using assms apply(induction hist)
-  apply(simp add: map_filter_simps(2))
+  apply(simp add: filter_bcast_def map_filter_simps(2))
   apply(case_tac a, case_tac "x1=msg")
   apply(metis list.set_intros(1))
-  apply(simp_all add: map_filter_simps(1))
+  apply(simp_all add: filter_bcast_def map_filter_simps(1))
 done
 
 lemma (in cbcast_protocol) broadcasts_history_eq:
   shows "Broadcast msg \<in> set (history i) \<longleftrightarrow> msg \<in> set (broadcasts i)"
   apply(rule iffI, simp add: broadcasts_def map_filter_def, force)
-  apply(simp add: broadcasts_def map_filter_broadcast)
+  apply(simp add: broadcasts_def filter_bcast_def map_filter_broadcast)
 done
 
 lemma (in cbcast_protocol) broadcast_node_id:
   assumes "Broadcast msg \<in> set (history i)"
-    and "msg_id msg = (j, seq)"
-  shows "i = j"
+  shows "fst (msg_id msg) = i"
   using assms apply -
   apply(subgoal_tac "\<exists>es1 es2. history i = es1 @ Broadcast msg # es2 \<and> Broadcast msg \<notin> set es1")
   prefer 2 apply(meson split_list_first)
@@ -187,48 +185,87 @@ lemma (in cbcast_protocol) broadcast_node_id:
   apply(metis fst_conv select_convs(1))
 done
 
-lemma (in cbcast_protocol) broadcast_msgid_increase:
-  assumes "history i = es1 @ [Broadcast m1] @ es2 @ [Broadcast m2] @ es3"
-    and "Broadcast m1 \<notin> set es1"
-  shows "snd (msg_id m1) < snd (msg_id m2)"
-  using assms apply -
-  apply(insert broadcast_origin, erule_tac x=i in meta_allE)
-  apply(erule_tac x=es1 in meta_allE, erule_tac x=m1 in meta_allE)
-  apply(erule_tac x="es2 @ [Broadcast m2] @ es3" in meta_allE)
-  apply(simp, ((erule exE)+, (erule conjE)+)+)
-  apply(subgoal_tac "\<exists>suf. fst (ba i) @ suf = fst (snd config i)") defer
-  apply(insert history_monotonic)[1]
-  apply(erule_tac x="config" in meta_allE)
-  apply(erule_tac x="pre @ [(a, b)]" in meta_allE)
-  apply(erule_tac x="(aa, ba)" in meta_allE)
-  apply(erule_tac x="suf" in meta_allE, erule_tac x="i" in meta_allE, simp)
-  apply(erule exE)
-  apply(subgoal_tac "sufa=es3") defer
-  apply(simp add: history_def)
-  (*apply(subgoal_tac "Broadcast m2 \<in> set (history i)") defer apply force
-  apply(drule broadcast_origin, (erule exE)+, (erule conjE)+)*)
-  oops
-
 lemma (in cbcast_protocol) broadcast_msg_id:
-  assumes "broadcasts i = pre @ [msg] @ suf"
-    shows "msg_id msg = (i, Suc (length pre))"
-  using assms apply(simp add: broadcasts_def)
+  assumes "history i = pre @ [Broadcast msg] @ suf"
+      and "Broadcast msg \<notin> set pre"
+    shows "msg_id msg = (i, Suc (length (filter_bcast pre)))"
+  using assms valid_execution apply simp
+  apply(frule config_evolution_exists, erule exE)
   apply(subgoal_tac "Broadcast msg \<in> set (history i)") defer
   using map_filter_broadcast apply force
-  apply(drule broadcast_origin, (erule exE)+, (erule conjE)+)
-  apply(subgoal_tac "Broadcast.broadcasts (snd before i) = pre")
+  apply(drule broadcast_origin, simp, (erule exE)+)
   apply(simp add: next_msgid_def)
-  apply(subgoal_tac "\<exists>es. history i = fst (snd before i) @ [Broadcast msg, Deliver msg] @ es")
+done
 
-  apply(insert Broadcast.broadcasts_def)
-  apply(erule_tac x="snd before i" in meta_allE)
-  using assms(1) apply -
-  apply(frule broadcasts_to_history, (erule exE)+, (erule conjE)+)
-  oops
+lemma bcast_append_length:
+  shows "length (filter_bcast (xs @ ys)) =
+     length (filter_bcast (xs)) + length (filter_bcast (ys))"
+by(simp add: filter_bcast_def map_filter_append)
+
+lemma (in cbcast_protocol) msg_id_distinct:
+  assumes "Broadcast m1 \<in> set (history j)"
+    and "Broadcast m2 \<in> set (history j)"
+    and "msg_id m1 = msg_id m2"
+  shows "m1 = m2"
+  using assms apply -
+  apply(drule_tac x="Broadcast m1" in list_first_index)
+  apply(drule_tac x="Broadcast m2" in list_first_index)
+  apply((erule_tac exE)+, (erule_tac conjE)+)
+  apply(subgoal_tac "msg_id m1 = (j, Suc (length (filter_bcast pre)))")
+  prefer 2 apply(metis broadcast_msg_id)
+  apply(subgoal_tac "msg_id m2 = (j, Suc (length (filter_bcast prea)))")
+  prefer 2 apply(metis broadcast_msg_id)
+  apply(subgoal_tac "length (filter_bcast pre) = length (filter_bcast prea)")
+  prefer 2 apply simp
+  apply(case_tac "i = ia", fastforce)
+  apply(case_tac "i < ia")
+  apply(subgoal_tac "\<exists>ms. prea = pre @ [Broadcast m1] @ ms", erule exE)
+  apply(subgoal_tac "length (filter_bcast prea) =
+    length (filter_bcast pre) + 1 + length (filter_bcast ms)", linarith)
+  apply(subgoal_tac "length (filter_bcast [Broadcast m1]) = 1")
+  prefer 2 apply(simp add: filter_bcast_def map_filter_def)
+  apply(metis (no_types, lifting) bcast_append_length add.assoc)
+  apply(subgoal_tac "pre = take i (history j)")
+  prefer 2 apply(simp add: append_eq_conv_conj)
+  apply(subgoal_tac "prea = take ia (history j)")
+    prefer 2 apply fastforce
+  apply(subgoal_tac "ia-i-1 \<ge> 0") prefer 2 apply blast
+  apply(rule_tac x="take (ia-i-1) suf" in exI)
+  apply(metis append.left_neutral append_Cons diff_is_0_eq diffs0_imp_equal
+    less_imp_le_nat take_Cons' take_all take_append)
+  apply(subgoal_tac "\<exists>ms. pre = prea @ [Broadcast m2] @ ms", erule exE)
+  apply(subgoal_tac "length (filter_bcast pre) =
+    length (filter_bcast prea) + 1 + length (filter_bcast ms)", linarith)
+  apply(subgoal_tac "length (filter_bcast [Broadcast m2]) = 1")
+  prefer 2 apply(simp add: filter_bcast_def map_filter_def)
+  apply(metis (no_types, lifting) bcast_append_length add.assoc)
+  apply(subgoal_tac "pre = take i (history j)")
+  prefer 2 apply(simp add: append_eq_conv_conj)
+  apply(subgoal_tac "prea = take ia (history j)")
+    prefer 2 apply fastforce
+  apply(subgoal_tac "i-ia-1 \<ge> 0") prefer 2 apply blast
+  apply(rule_tac x="take (i-ia-1) sufa" in exI)
+  apply(metis One_nat_def Suc_diff_Suc append_Cons append_Nil diff_zero less_imp_le_nat
+    linorder_neqE_nat take_Suc_Cons take_all take_append zero_less_diff)
+done
+
+lemma (in cbcast_protocol) msg_id_unique:
+  assumes "Broadcast m1 \<in> set (history i)"
+      and "Broadcast m2 \<in> set (history j)"
+      and "msg_id m1 = msg_id m2"
+    shows "i = j \<and> m1 = m2"
+  using assms apply -
+  apply(case_tac "i=j")
+  using msg_id_distinct apply blast
+  apply(subgoal_tac "fst (msg_id m1) = i")
+  apply(subgoal_tac "fst (msg_id m2) = j", force)
+  using broadcast_node_id apply fastforce+
+done
 
 context cbcast_protocol begin
 sublocale causal: causal_network history msg_id
   apply standard
+  prefer 4 apply(simp add: msg_id_unique)
   oops
 
 end
